A12Kernel.lean
@@ -100,6 +100,7 @@ import A12Kernel.Elaboration.NumericComputation
 import A12Kernel.Elaboration.StringComputation
 import A12Kernel.Elaboration.StringComputationTable
 import A12Kernel.Elaboration.StringComputationRun
+import A12Kernel.Elaboration.StringComputationRunRelation
 import A12Kernel.Elaboration.EnumerationComputation
 import A12Kernel.Elaboration.EnumerationFirstFilledComputation
 import A12Kernel.Elaboration.NumericValidation
